Gets ugly when  non-aligned

proof/correctness/avx2/MLKEM_Poly_avx2_proof_mr.ec
@@ -226,7 +226,13 @@ qed.
 op lane_func_csubq(x : W16.t) = if W16.of_int 3329 \sle x then x - W16.of_int 3329 else x. 
 op pre16_csubq(x : W16.t) : bool =  W16.zero \sle x && x \slt W16.of_int (6658). 
 
-
+lemma post_commutes_csubq x : pre16_csubq x =>
+    incoeff (to_sint x) = incoeff (to_sint (lane_func_csubq x)) /\ bpos16 (lane_func_csubq x) q.
+proof.
+rewrite /pre16_csubq /lane_func_csubq sltE !sleE /= /smod /= -eq_incoeff. 
+case (3329 <= to_sint x);last by smt().
+by move => *;rewrite  to_sintB_small /= /smod /= /#. 
+qed.
 
 lemma poly_csubq_corr_h ap :
       hoare[ Jkem_avx2.M(Syscall)._poly_csubq :
@@ -235,7 +241,7 @@ lemma poly_csubq_corr_h ap :
              ==>
              ap = lift_array256 res /\
              pos_bound256_cxq res 0 256 1 ].
-proc. 
+proc.
   proc rewrite 1  sliceget_256_16_16E.
   unroll for 3. 
   proc rewrite 3  sliceget_256_256_16E.
@@ -283,31 +289,22 @@ proc.
          pre16_csubq _ _);
    [ by move => x; rewrite /pre16_csubq sleE sltE /=   /to_sint /smod /= qE //= | by smt() ]. 
   
-move => &hr WRONG_POST.
+rewrite /lift_array256 /pos_bound256_cxq;move => &hr [#] H H0 rp0new WRONG_POST.
 have PRE : 
-(_rp0 = rp{hr} /\ pos_bound256_cxq _rp0 0 256 2) /\
-  map lane_func_csubq (map W16.bits2w (chunk 16 (flatten [flatten (map W16.w2bits (to_list _rp0))]))) =
-  map W16.bits2w (chunk 16 (flatten [flatten (map W16.w2bits (to_list rp{hr}))])). 
+map lane_func_csubq (map W16.bits2w (chunk 16 (flatten [flatten (map W16.w2bits (to_list _rp0))]))) =
+            map W16.bits2w (chunk 16 (flatten [flatten (map W16.w2bits (to_list rp0new{hr}))])). 
 apply WRONG_POST.
 clear WRONG_POST.  
-have : forall k, nth witness (map lane_func_csubq (map W16.bits2w (chunk 16 (flatten [flatten (map W16.w2bits (to_list _rp0))])))) k =
-     nth witness (map W16.bits2w (chunk 16 (flatten [flatten (map W16.w2bits (to_list rp{hr}))]))) k by smt().
-move => Hk;rewrite /lift_array256 /pos_bound256_cxq tP;split => i ib /=.
-rewrite !mapiE //=.
-move : (Hk i).
-rewrite get_vs_bits_256u16 //=.
-rewrite (nth_map witness); 1: by smt(size_map get_vs_bits_256u16_size).
-rewrite get_vs_bits_256u16 //=.
-rewrite /lane_func_csubq sleE /= /smod /= -eq_incoeff. 
-case (3329 <= to_sint _rp0.[i]);last by smt().
-by move => ? <-; rewrite  to_sintB_small /= /smod /= /#.
-move : (Hk i).
-rewrite get_vs_bits_256u16 //=.
-rewrite (nth_map witness); 1: by smt(size_map get_vs_bits_256u16_size).
-rewrite get_vs_bits_256u16 //=.
-rewrite /lane_func_csubq  sleE /= /smod /= qE.
-case (3329 <= to_sint _rp0.[i]);last by smt(). 
-by move => ? <-; rewrite  to_sintB_small /= /smod /= /#.
+have HH  : forall k, nth witness (map lane_func_csubq (map W16.bits2w (chunk 16 (flatten [flatten (map W16.w2bits (to_list _rp0))])))) k = nth witness (map W16.bits2w (chunk 16 (flatten [flatten (map W16.w2bits (to_list rp0new))]))) k by smt().
+rewrite Array256.tP;split => k kb.
++ rewrite !Array256.mapiE //=;move : (HH k).
+  rewrite (nth_map witness);1: smt(size_map get_vs_bits_256u16_size). 
+  rewrite !get_vs_bits_256u16 1,2:/#. 
+  by smt(post_commutes_csubq pow2_16 W16.of_uintK W16.to_uintK ).
+move : (HH k).
+rewrite  (nth_map witness)  /=;1: smt(size_map get_vs_bits_256u16_size).
+have?: 2^(16-1) = 32768 by auto. 
+by smt(post_commutes_csubq get_vs_bits_256u16 pow2_16  W16.of_uintK W16.to_uintK ).
 qed.
  
 lemma poly_csubq_ll : islossless Jkem_avx2.M(Syscall)._poly_csubq.
@@ -350,12 +347,29 @@ op compress_alt (d : int) (c : coeff) : int =
 op sliceget_4_64 (bw: W64.t) (i: int) : W4.t = W4.bits2w (W64.w2bits bw).
 
 
-op lane_func_compress1(x : W16.t) : W4.t = sliceget_4_64 ((((W4u16.zeroextu64 x) `<<` W8.of_int 4) + W64.of_int (1665)) * (W64.of_int (80635) `>>` W8.of_int 28)) 0. 
-
 op lane_func_compress(x : W16.t) : W4.t = sliceget_4_64 (
    (((W4u16.zeroextu64 x) `<<` W8.of_int 4) + W64.of_int 1665) * (W64.of_int 80635) `>>` W8.of_int 28) 0. 
 
 op pre16_compress(x : W16.t) : bool =  W16.zero \sle x && x \slt W16.of_int (3329). 
+
+
+lemma post_commutes_compress x : pre16_compress x =>
+    to_uint (lane_func_compress x) = compress_alt 4 (incoeff (to_sint x)).
+admitted.
+
+require import EncDecCorrectness.
+
+op encode (l : int, ints : int list) : bool list = 
+  flatten (map (BitEncoding.BS2Int.int2bs l) ints). 
+
+op BitsToBytes(bits : bool list) : W8.t list = (map W8.bits2w (chunk 8 bits)).
+
+op sem_encode4 (a : int Array256.t) : W8.t Array128.t = Array128.of_list W8.zero (BitsToBytes (encode 4  (to_list a))).
+
+lemma sem_encode4_corr: sem_encode4 = encode4.
+proof. 
+rewrite /sem_encode4 /encode4 fun_ext => x /=.
+admitted.
 
 lemma poly_compress_1_corr_mr_h _a mem :
     hoare [ Jkem_avx2.M(Syscall)._poly_compress_1  :
@@ -368,7 +382,6 @@ lemma poly_compress_1_corr_mr_h _a mem :
              pos_bound256_cxq res.`2 0 256 1 /\
              res.`1 = encode4 (compress_poly 4 _a)].
 proof.
-rewrite /compress_poly. have ->  : (compress 4) = (compress_alt 4).  smt(fun_ext compress_alt_compress). 
 proc. 
 seq 2 : (pos_bound256_cxq a 0 256 1 /\ lift_array256 a = _a /\ Glob.mem = mem); 1:by call (poly_csubq_corr_h _a); auto => /> /#.
 cfold 7.
@@ -396,10 +409,13 @@ proc rewrite 54 sliceset_256_128_8E.
 proc rewrite 78 sliceset_256_128_8E.
 proc rewrite 102 sliceset_256_128_8E.
 cfold 7.
-conseq />.
+conseq />.  
   exists * a ;elim * =>_aw.
   conseq (: _aw = a /\ pos_bound256_cxq _aw 0 256 1 ==> 
-          rp = encode4 (map (compress_alt 4) (lift_array256 _aw)));1,2: smt(). 
+          rp = sem_encode4 (map (compress_alt 4) (lift_array256 _aw))); 1:smt().
++ move => &hr [#] *. 
+  rewrite -sem_encode4_corr /compress_poly.
+  by have -> /# : (compress 4) = (compress_alt 4); 1: by rewrite fun_ext => *;smt(compress_alt_compress).
 
 bdep 16 4 [ "_aw" ] [ "a" ] [ "rp" ] lane_func_compress pre16_compress.
 
@@ -409,33 +425,95 @@ bdep 16 4 [ "_aw" ] [ "a" ] [ "rp" ] lane_func_compress pre16_compress.
          pre16_compress _ _);
    [ by move => x; rewrite /pre16_compress sleE sltE /=   /to_sint /smod /= qE //= | by smt() ]. 
   
-move => &hr WRONG_POST.
+move => &hr [#] H H0 newrp0 WRONG_POST.
 have PRE : 
-((_aw = a{hr} /\ pos_bound256_cxq _aw 0 256 1) /\
-            map lane_func_compress (map W16.bits2w (chunk 16 (flatten [flatten (map W16.w2bits (to_list _aw))]))) =
-            map W4.bits2w (chunk 4 (flatten [flatten (map W8.w2bits (to_list rp{hr}))]))). 
+map lane_func_compress (map W16.bits2w (chunk 16 (flatten [flatten (map W16.w2bits (to_list _aw))]))) =
+map W4.bits2w (chunk 4 (flatten [flatten (map W8.w2bits (to_list newrp0))])). 
 apply WRONG_POST.
 clear WRONG_POST.  
-have : forall k, nth witness (map lane_func_compress (map W16.bits2w (chunk 16 (flatten [flatten (map W16.w2bits (to_list _aw))])))) k =
-     nth witness (map W4.bits2w (chunk 4 (flatten [flatten (map W8.w2bits (to_list rp{hr}))]))) k by smt().
-move => Hk;rewrite /lift_array256 /pos_bound256_cxq tP => i ib /=.
-move : (Hk i).
+rewrite /sem_encode4 /=. 
+have HH : forall k, nth witness (map lane_func_compress (map W16.bits2w (chunk 16 (flatten [flatten (map W16.w2bits (to_list _aw))])))) k =
+     nth witness (map W4.bits2w (chunk 4 (flatten [flatten (map W8.w2bits (to_list newrp0))]))) k by smt().
+rewrite Array128.tP => k kb; rewrite get_of_list // /BitsToBytes /encode.
+move : (HH (2*k)).
+rewrite (nth_map witness); 1: by  smt(size_map get_vs_bits_256u16_size).
+rewrite get_vs_bits_256u16 1:/#. 
+rewrite (nth_map witness); 1: by  smt(size_map get_vs_bits_256u16_size).
+rewrite flatten1 (nth_map witness) /=.
++ rewrite size_iota size_flatten -map_comp /(\o) /=. 
+  have -> : map (fun (_ : W8.t) => 8) (to_list newrp0) =
+               mkseq (fun _ => 8) 128; last by
+        rewrite /mkseq -iotaredE /= /sumz /= /#. 
+     apply (eq_from_nth witness).
+     + by rewrite size_map Array128.size_to_list size_mkseq /#.
+     move => i.
+     rewrite size_map Array128.size_to_list => ib.
+     rewrite (nth_map witness) /=;1: by smt(Array128.size_to_list).
+     by rewrite (nth_mkseq) /#.
+rewrite nth_iota /=. admit.
+have -> : 4 * (2 * k) = 8 * k by ring.
+rewrite drop_flatten_ctt. admit. 
+rewrite -map_drop. 
+have /= <- := take_take ((flatten (map W8.w2bits (drop k (to_list newrp0))))) 4 8.
+have -> : (take 8 (flatten (map W8.w2bits (drop k (to_list newrp0))))) = 
+             W8.w2bits newrp0.[k]. admit.
+move => HH2k.
+
+move : (HH (2*k+1)).
+rewrite (nth_map witness); 1: by  smt(size_map get_vs_bits_256u16_size).
+rewrite get_vs_bits_256u16 1:/#. 
+rewrite (nth_map witness); 1: by  smt(size_map get_vs_bits_256u16_size).
+rewrite flatten1 (nth_map witness) /=.
++ rewrite size_iota size_flatten -map_comp /(\o) /=. 
+  have -> : map (fun (_ : W8.t) => 8) (to_list newrp0) =
+               mkseq (fun _ => 8) 128; last by
+        rewrite /mkseq -iotaredE /= /sumz /= /#. 
+     apply (eq_from_nth witness).
+     + by rewrite size_map Array128.size_to_list size_mkseq /#.
+     move => i.
+     rewrite size_map Array128.size_to_list => ib.
+     rewrite (nth_map witness) /=;1: by smt(Array128.size_to_list).
+     by rewrite (nth_mkseq) /#.
+rewrite nth_iota /=. admit.
+have -> : 4 * (2 * k + 1) = 4 + 8*k by ring.
+rewrite -drop_drop 1,2:/#.
+rewrite drop_flatten_ctt. admit. 
+rewrite -map_drop. 
+have -> : (drop 4 (flatten (map W8.w2bits (drop k (to_list newrp0))))) = 
+      (drop 4 (take 8 (flatten (map W8.w2bits (drop k (to_list newrp0)))))).
++ apply (eq_from_nth witness). admit.  admit.
+have -> : (take 8 (flatten (map W8.w2bits (drop k (to_list newrp0))))) = 
+             W8.w2bits newrp0.[k]. admit.
+rewrite {1}(:4 = size (drop 4 (w2bits newrp0.[k]))). admit. 
+rewrite take_size.
+move => HH2k1.
+
+rewrite (nth_map witness).
++    rewrite size_chunk // size_flatten // -map_comp /(\o). 
+     rewrite (eq_map _ (fun _ => 4)) => //=;1: smt(BitEncoding.BS2Int.size_int2bs).
+     have -> : map (fun (_ : int) => 4) (to_list (map (compress_alt 4) (lift_array256 _aw))) =
+               mkseq (fun _ => 4) 256; last 
+        by rewrite /mkseq -iotaredE /= /sumz /=. 
+     apply (eq_from_nth witness).
+     + by rewrite size_map Array256.size_to_list size_mkseq /#.
+     move => i.
+     rewrite size_map Array256.size_to_list => ib.
+     rewrite (nth_map witness) /=;1: by smt(Array256.size_to_list).
+     by rewrite (nth_mkseq) /#.
+rewrite (nth_map witness) /=.
++ rewrite size_iota size_flatten -map_comp /(\o) /=.
+  have -> : (map (fun (x : int) => size ((BitEncoding.BS2Int.int2bs 4 x)))
+        (to_list (map (compress_alt 4) (lift_array256 _aw)))) =
+               mkseq (fun _ => 4) 256; last by
+        rewrite /mkseq -iotaredE /= /sumz /= /#. 
+     apply (eq_from_nth witness).
+     + by rewrite size_map Array256.size_to_list size_mkseq /#.
+     move => i.
+     rewrite size_map Array256.size_to_list => ib.
+     rewrite (nth_map witness) /=;1: by smt(Array256.size_to_list).
+     by rewrite (nth_mkseq);smt(BitEncoding.BS2Int.size_int2bs).
+rewrite nth_iota /=. admit.
 admit.
-(* 
-rewrite get_vs_bits_256u16 //=.
-rewrite (nth_map witness); 1: by smt(size_map get_vs_bits_256u16_size).
-rewrite get_vs_bits_256u16 //=.
-rewrite /lane_func_csubq sleE /= /smod /= -eq_incoeff. 
-case (3329 <= to_sint _rp0.[i]);last by smt().
-by move => ? <-; rewrite  to_sintB_small /= /smod /= /#.
-move : (Hk i).
-rewrite get_vs_bits_256u16 //=.
-rewrite (nth_map witness); 1: by smt(size_map get_vs_bits_256u16_size).
-rewrite get_vs_bits_256u16 //=.
-rewrite /lane_func_csubq  sleE /= /smod /= qE.
-case (3329 <= to_sint _rp0.[i]);last by smt(). 
-by move => ? <-; rewrite  to_sintB_small /= /smod /= /#.
-*)
 qed.
 
 
